\message{ !name(ParallelResumen.tex)}\documentclass{article} 


\usepackage[hidelinks]{hyperref}
\usepackage[references,links]{agda}
\usepackage{amsmath}
\usepackage{amsthm}
\usepackage{mathtools}
\usepackage{textgreek}
\usepackage{catchfilebetweentags}
\usepackage{tipa}
\usepackage{graphicx}
\usepackage{bussproofs}

%math
\newcommand{\alp}{\ensuremath{\alpha}}
\newcommand{\lamb}{\ensuremath{\lambda}}
\newcommand{\alpsym}{\ensuremath{\sim_\alpha}}
\newcommand{\choice}{\ensuremath{\chi}}
\newcommand{\p}{\ensuremath{\rightrightarrows}}

%Agda
\newcommand{\freshin}[2]{\ensuremath{#1 \mathbin{\AgdaDatatype{\#}} #2}}
\newcommand{\lambAg}[2]{\ensuremath{\AgdaInductiveConstructor{ƛ}\, #1\, #2}}
\newcommand{\inAg}{\ensuremath{\mathbin{\AgdaFunction{∈}}}}
\newcommand{\ninAg}{\ensuremath{\mathbin{\AgdaFunction{∉}}}}
\newcommand{\neqAg}{\ensuremath{\mathbin{\AgdaInductiveConstructor{≢}}}}
\newcommand{\ap}[2]{#1 \ensuremath{\mathbin{\AgdaInductiveConstructorFunction{·}} #2}}
\newcommand{\var}[1]{\ensuremath{\AgdaInductiveConstructorFunction{v}\, #1}}
\newcommand{\fv}{\ensuremath{{\AgdaFunction{fv}}\,}}
\newcommand{\perm}{\ensuremath{\mathbin{\AgdaFunction{∙}}}}
\newcommand{\perma}{\ensuremath{\mathbin{\AgdaFunction{∙}_a}}}
\newcommand{\free}{\ensuremath{\mathbin{\AgdaFunction{*}}}}
\newcommand{\choiceAg}{\ensuremath{\AgdaFunction{χ}\,}}
\newcommand{\choiceAgaux}{\ensuremath{\AgdaFunction{χ'}\,}}
\newcommand{\alpeqAg}{\ensuremath{\mathbin{\AgdaDatatype{∼α}}}}
\newcommand{\swap}[3]{\ensuremath{(#1 \mathbin{\AgdaFunction{∙}} #2)\, #3}}

\newcommand{\betaalpha}{\ensuremath{\rightarrow_\alpha}}
\newcommand{\betaaster}{\ensuremath{\rightarrow_\beta^*}}
\newcommand{\lam}{\ensuremath{\lambda}}
\newcommand{\conc}{\ensuremath{\mathop{+\!\!+}}}


% \newcommand{\agdaf}[1]{\ensuremath{\AgdaFunction{#1}\,}}
% \newcommand{\agdaD}[1]{\ensuremath{\AgdaDatatype{#1}\,}}
% \newcommand{\agdav}[1]{\ensuremath{\AgdaBound{#1}\,}}

\DeclareUnicodeCharacter{411}{\textipa{\textcrlambda}}
\DeclareUnicodeCharacter{65288}{(}
\DeclareUnicodeCharacter{65289}{)}
\DeclareUnicodeCharacter{8788}{\ensuremath{\coloneqq}}
\DeclareUnicodeCharacter{8336}{\ensuremath{_a}}
\DeclareUnicodeCharacter{8799}{\ensuremath{\overset{?}{=}}}
\DeclareUnicodeCharacter{8759}{\ensuremath{\dblcolon}}
\DeclareUnicodeCharacter{8718}{\ensuremath{\square}}

\newtheorem{lem}{Lemma}

\begin{document}

\message{ !name(ParallelResumen.tex) !offset(-1) }
alpha}

\begin{minipage}{0.2\linewidth}
  \AxiomC{$$} \LeftLabel{\alpsym v} \UnaryInfC{$x \alpsym x$} \DisplayProof
\end{minipage}
\begin{minipage}{0.4\linewidth}
  \AxiomC{$M \alpsym M'$} 
  \AxiomC{$N \alpsym N'$}
  \LeftLabel{\alpsym a}
  \BinaryInfC{$M N \alpsym M' N'$} \DisplayProof
\end{minipage}
\begin{minipage}{0.4\linewidth}
  \AxiomC{$\exists xs, \forall z \not\in xs, (x\ z) M \alpsym (y\ z) N$} 
    \LeftLabel{\alpsym \lam}
  \UnaryInfC{$\lambda x M  \alpsym  \lambda y N$} \DisplayProof
\end{minipage}


\section{Parallel Reduction}\label{parallel}


\begin{minipage}{0.2\linewidth}
  \AxiomC{$$}   \LeftLabel{\p v} \UnaryInfC{$x \p x$} \DisplayProof
\end{minipage}
\begin{minipage}{0.4\linewidth}
  \AxiomC{$M \p M'$} 
  \AxiomC{$N \p N'$}
  \LeftLabel{\p a}
  \BinaryInfC{$M N \p M' N'$} \DisplayProof
\end{minipage}
\begin{minipage}{0.4\linewidth}
  \AxiomC{$\exists xs, \forall z \not\in xs, (x\ z) M \p (y\ z) N$} 
  \LeftLabel{\p \lam}
  \UnaryInfC{$\lambda x M  \p  \lambda y N$} \DisplayProof
\end{minipage}

\begin{center}
  \AxiomC{$\lambda x M \p \lambda y P'$}
  \AxiomC{$N \p  P''$}
  \AxiomC{$P \alpsym P' [y := P'']$}
  \LeftLabel{$\p \beta$}
  \TrinaryInfC{$(\lambda x M) N  \p P$}
  \DisplayProof
\end{center}

\begin{lem}[Parallel is equivariant]
\label{pequiv}
\[ M \p N \Rightarrow \pi M \p \pi N \]
\end{lem}

\begin{proof}
Induction on the parallel relation.

\begin{itemize}
   \item[var. rule:] Direct.
   \item[app. rule:] Direct.
   \item[\lam\ rule:] 
\begin{minipage}{0.2\linewidth}
     Hypotheses:
\end{minipage}
\begin{minipage}{0.4\linewidth}
  \AxiomC{$\exists xs, \forall z \not\in xs, (x\ z) M \p (y\ z) N$} 
  \LeftLabel{\p \lam}
  \UnaryInfC{$\lambda x M  \p  \lambda y N$} \DisplayProof
\end{minipage}

Thesis:  $\lambda (\pi\ x) (\pi\ M)  \p  \lambda (\pi\ y) (\pi\ N)$

Proof:


  \AxiomC{$\exists xs, \forall z \not\in xs, (x\ z) M \p (y\ z) N$} 
  \UnaryInfC{$\forall z \not\in xs \conc dom(\Gamma), (x\ z) M \p (y\ z) N$} 
  \LeftLabel{ih}
  \UnaryInfC{$\forall z \not\in xs \conc dom(\Gamma), \pi ((x\ z) M) \p \pi ((y\ z) N)$} 
  \UnaryInfC{$\forall z \not\in xs \conc dom(\Gamma),  ((\pi\ x)\ (\pi\ z)) (\pi\ M) \p  ((\pi\ y)\ (\pi\ z)) (\pi\ N)$} 
  \LeftLabel{$(\pi\ z) \equiv z\ as\ z \not\in dom(\Gamma) $}
  \UnaryInfC{$ \forall z \not\in xs \conc dom(\Gamma), ((\pi\ x)\ z) (\pi\ M) \p ((\pi\ y)\ z) (\pi\ N)$} 
  \LeftLabel{\p \lam}
  \UnaryInfC{$\lambda (\pi\ x) (\pi\ M)  \p  \lambda (\pi\ y) (\pi\ N)$} \DisplayProof


   \item[$\beta$\ rule:]
\begin{minipage}{0.2\linewidth}
     Hypotheses:
\end{minipage}
\begin{minipage}{0.4\linewidth}
  \AxiomC{$\lambda x M \p \lambda y P'$}
  \AxiomC{$N \p  P''$}
  \AxiomC{$P \alpsym P' [y := P'']$}
  \LeftLabel{$\p \beta$}
  \TrinaryInfC{$(\lambda x M) N  \p P$}
  \DisplayProof
\end{minipage}

Thesis:  $(\lambda (\pi\ x) (\pi\ M)) (\pi\ N)  \p \pi\ P$

Proof:


  \AxiomC{$\lambda x M \p \lambda y P'$}
  \LeftLabel{ih}
  \UnaryInfC{$\lambda (\pi\ x) (\pi\ M) \p \lambda (\pi\ y) (\pi\ P')$}
  \AxiomC{$N \p  P''$}
  \LeftLabel{ih}
  \UnaryInfC{$\pi\ N \p  \pi\ P''$}
  \AxiomC{$ P \alpsym P' [y := P'']$}
  \LeftLabel{\alp\ equiv.}
  \UnaryInfC{$\pi\ P \alpsym \pi\ (P' [y := P''])$}
  \LeftLabel{\alp\ ind.}
  \UnaryInfC{$\pi\ P \alpsym (\pi\ P') [ (\pi\ y) := (\pi\ P'')]$}
  \LeftLabel{$\p \beta$}
  \TrinaryInfC{$(\lambda (\pi\ x) (\pi\ M)) (\pi\ N)  \p \pi\ P$}
  \DisplayProof
\end{itemize}
\end{proof}

\begin{lem}[Parallel is right \alp-equivalent]
\label{prightalpha}
\[ M \p N \wedge N \alpsym P \Rightarrow M \p P \]
\end{lem}

\begin{proof}
Trivial induction on the parallel relation.

\begin{itemize}
   \item[var. rule:] Direct.
   \item[app. rule:] Direct.
   \item[\lam\ rule:] 

     Hypotheses: 

\begin{minipage}{0.5\linewidth}
  \AxiomC{$\exists xs, \forall z \not\in xs, (x\ z) M \p (y\ z) N$} 
  \LeftLabel{\p \lam}
  \UnaryInfC{$\lambda x M  \p  \lambda y N$} \DisplayProof
\end{minipage}
\begin{minipage}{0.5\linewidth}
  \AxiomC{$\exists ys, \forall w \not\in xs, (y\ w) N \alpsym (z\ w) P$} 
  \LeftLabel{\alpsym a}
  \UnaryInfC{$\lambda y N  \alpsym   \lambda z P$} \DisplayProof
\end{minipage}

Thesis:  $\lambda x M  \p  \lambda z P$

Proof:
  \AxiomC{$\forall w \not\in xs \conc ys, (x\ w) M \p (y\ w) N$} 
  \AxiomC{$\forall w \not\in xs \conc ys, (y\ w) N \alpsym (z\ w) P$} 
  \LeftLabel{ih}
  \BinaryInfC{$\forall w \not\in xs \conc ys, (x\ w) M \p (z\ w) P$} 
  \LeftLabel{\p \lam}
  \UnaryInfC{$\lambda x M  \p  \lambda z P$} \DisplayProof


   \item[$\beta$\ rule:]
\begin{minipage}{0.2\linewidth}
     Hypotheses: 
\end{minipage}

\begin{minipage}{0.8\linewidth}
  \AxiomC{$\lambda x M \p \lambda y P'$}
  \AxiomC{$N \p  P''$}
  \AxiomC{$P \alpsym P' [y := P'']$}
  \LeftLabel{$\p \beta$}
  \TrinaryInfC{$(\lambda x M) N  \p P$}
  \DisplayProof
\end{minipage}
\begin{minipage}{0.1\linewidth}
  \[ P \alpsym Q  \]
\end{minipage}

Thesis:  $(\lambda x M) N \p Q$

Proof:

  \AxiomC{$\lambda x M \p \lambda y P'$}
  \AxiomC{$N \p  P''$}
  \AxiomC{$Q \alpsym P \alpsym P' [y := P'']$}
  \UnaryInfC{$Q \alpsym P' [y := P'']$}
  \LeftLabel{$\p \beta$}
  \TrinaryInfC{$(\lambda x M) N  \p P$}
  \DisplayProof
\end{itemize}
\end{proof}

\begin{lem}[Parallel is left \alp-equivalent]
\label{pleftalpha}
\[ M \alpsym N \wedge N \p P \Rightarrow M \p P \]
\end{lem}

\begin{proof}
Trivial induction on the parallel relation, analog to previous one as rules are symetric except from the $\beta$ rule that we discuss next.

\begin{itemize}

   \item[$\beta$\ rule:]
\begin{minipage}{0.2\linewidth}
     Hypotheses: 
\end{minipage}

\begin{minipage}{0.22\linewidth}
  \[ Q \alpsym (\lambda x M) N \]
\end{minipage}
\begin{minipage}{0.78\linewidth}
  \AxiomC{$\lambda x M \p \lambda y P'$}
  \AxiomC{$N \p  P''$}
  \AxiomC{$P \alpsym P' [y := P'']$}
  \LeftLabel{$\p \beta$}
  \TrinaryInfC{$(\lambda x M) N  \p P$}
  \DisplayProof
\end{minipage}

Thesis:  $Q \p P$

Proof:

  \[ Q \alpsym (\lambda x M) N  \Rightarrow Q \equiv(\lam y Q') Q'' \wedge \lam z Q' \alpsym \lambda x M \wedge Q'' \alpsym  N\]

  \AxiomC{$\lam z Q' \alpsym \lambda x M$}
  \AxiomC{$\lambda x M \p \lambda y P'$}
  \LeftLabel{hi}
  \BinaryInfC{$\lam z Q'  \p  \lambda y P'$}

  \AxiomC{$Q'' \alpsym N$}
  \AxiomC{$N \p P''$}
  \LeftLabel{hi}
  \BinaryInfC{$Q'' \p P''$}

  \AxiomC{$P \alpsym P' [y := P'']$}
  \LeftLabel{$\p \beta$}
  \TrinaryInfC{$Q \p P$}
  \DisplayProof
\end{itemize}
\end{proof}

\begin{lem}[Parallel relation preserves freshness]
\label{pfresh}
\[ x \# M \wedge M \p N  \Rightarrow x \# N \]
\end{lem}


\begin{lem}[Parallel relation \lam-elimination]
\label{lamelim}
\[ \lam x M \p M' \Rightarrow (\exists M'')(M \p M'' , \lam x M \p \lam x M'' , M' \alpsym \lam x M'') \]
\end{lem}

\begin{proof}
We prove that $M'' = (y\ x) M'$\  satifies all conjunction assertions in the thesis.

As $\lam x M \p M'$\ by parallel elimination we know:
\begin{itemize}
\item $M' = \lam y M'$
\item $\exists xs, \forall z \not\in xs, (x\ z)M \p (y\ z) M'$
\end{itemize}

Next prove the thesis conjunctions:

\begin{itemize}
\item
  \AxiomC{be $z \not\in xs \cup fv (\lam y M')$}
  \AxiomC{$\forall z \not\in xs, (x\ z)M \p (y\ z) M'$}
  \BinaryInfC{$(x\ z) M \p (y\ z) M'$}
  \LeftLabel{\p\ equiv.}
  \UnaryInfC{$(x\ z) (x\ z) M \p (x\ z) (y\ z) M'$}
  \LeftLabel{swap idem.}
  \UnaryInfC{$ M \p (x\ z) (y\ z) M'$}
  \AxiomC{$x \# \lam y M'$}
  \AxiomC{$z \not\in fv (\lam y M')$}
  \UnaryInfC{$z \# \lam y M'$}
  \BinaryInfC{$(x\ z) (y\ z) M' \alpsym (x\ y) M'$}   
  \LeftLabel{lem.\ref{prightalpha}}
  \BinaryInfC{$M \p (x\ y) M'$}   
  \DisplayProof

\item
  \AxiomC{$\lam x M \p \lam y M'$}
  \AxiomC{$\lam y M' \alpsym \lam x ((x\ y) M')$}
  \LeftLabel{lem.\ref{prightalpha}}
  \BinaryInfC{$\lam x M \p \lam x ((x\ y) M')$}   
  \DisplayProof

\item
  \AxiomC{$x \# \lam x M$}
  \AxiomC{$\lam x M \p \lam y M'$}
  \LeftLabel{lem.\ref{pfresh}}
  \BinaryInfC{$x \# \lam y M'$}
  \UnaryInfC{$\lam y M' \alpsym \lam x ((y\ x) M')$}
  \DisplayProof

\end{itemize}
\end{proof}

\begin{lem}[Parallel relation $\beta$-elimination]
\label{betaelim}
\[ \lam x M \p \lam y M' , N \p N' , M' [ y := N' ] \alpsym P \Rightarrow (\exists M'')( \lam x M \p \lam x M'' , M'' [x := N'] \alpsym P) \]
\end{lem}

\begin{proof}
We prove that $M'' = (y\ x) M'$\  satifies both conjunction assertions in the thesis:

\begin{itemize}
\item 
  \AxiomC{$\lam x M \p \lam y M'$}
  \AxiomC{$x \# \lam x M$}
  \AxiomC{$\lam x M \p \lam y M'$}
  \LeftLabel{lem.\ref{pfresh}}
  \BinaryInfC{$x \# \lam y M'$}
  \UnaryInfC{$\lam y M' \alpsym \lam x ((x\ y) M')$}
  \LeftLabel{lem.\ref{prightalpha}}
  \BinaryInfC{$\lam x M \p \lam x ((y\ x) M')$}   
  \DisplayProof
\item

\[ \begin{array}{lcl}
      ((y\ x) M') [x := N'] &\alpsym& \text{} \\
      ((x\ y) M') [x := N'] &\alpsym& \text{lemma proved by alpha induction} \\
      M' [y := N'] &\alpsym& \text{hypothesis} \\
      P
   \end{array} \]

\end{itemize}
\end{proof}

\section{Other alpha primitive induction principle}
\label{sec:alphaprinciple}

\[
  \begin{array}{}
    P \alpha-
\message{ !name(ParallelResumen.tex) !offset(39) }

\end{document}